step2 step3 okay..

arm/proofs/bignum_add_inlined.ml
@@ -1,0 +1,2 @@
+open Hol_lib;;
+open Hol_loader;;
